src/Boolify/src/EncodeScript.sml
@@ -1,18 +1,69 @@
 (* Interactive mode
-app load ["listSyntax", "combinSyntax", "state_transformerTheory"];
+app load ["listSyntax", "combinSyntax", "rich_listTheory"];
 *)
 
-open HolKernel boolLib Parse bossLib pairSyntax numSyntax listSyntax
-  combinSyntax arithmeticTheory mesonLib simpLib boolSimps numLib
-  optionTheory oneTheory listTheory combinTheory state_transformerTheory
-  pairTheory;
+open HolKernel boolLib Parse bossLib pairTheory pairTools
+     arithmeticTheory listTheory rich_listTheory optionTheory;
+
+val REVERSE = Tactical.REVERSE;
 
 val _ = new_theory "Encode";
 
-infix 0 THEN |->;
-infixr 1 --> by;
+infixr 0 ++ || <<;
+infix 1 >>;
 
-val arith_ss = bool_ss ++ numSimps.ARITH_ss;
+val op ++ = op THEN;
+val op >> = op THEN1;
+val op << = op THENL;
+val op || = op ORELSE;
+
+val Suff = Q_TAC SUFF_TAC;
+val Know = Q_TAC KNOW_TAC;
+
+(*---------------------------------------------------------------------------
+        Theorems that should be somewhere else.
+ ---------------------------------------------------------------------------*)
+
+val IS_PREFIX_APPEND1 = store_thm
+  ("IS_PREFIX_APPEND1",
+   ``!a b c. IS_PREFIX c (APPEND a b) ==> IS_PREFIX c a``,
+   Induct >> RW_TAC std_ss [IS_PREFIX]
+   ++ RW_TAC std_ss []
+   ++ Cases_on `c`
+   ++ POP_ASSUM MP_TAC
+   ++ RW_TAC std_ss [IS_PREFIX, APPEND]
+   ++ PROVE_TAC []);
+
+val IS_PREFIX_APPEND2 = store_thm
+  ("IS_PREFIX_APPEND2",
+   ``!a b c. IS_PREFIX (APPEND b c) a ==> IS_PREFIX b a \/ IS_PREFIX a b``,
+   Induct >> RW_TAC std_ss [IS_PREFIX]
+   ++ RW_TAC std_ss []
+   ++ Cases_on `b` >> RW_TAC std_ss [IS_PREFIX]
+   ++ POP_ASSUM MP_TAC
+   ++ RW_TAC std_ss [IS_PREFIX, APPEND]
+   ++ PROVE_TAC []);
+
+val IS_PREFIX_APPENDS = store_thm
+  ("IS_PREFIX_APPENDS",
+   ``!a b c. IS_PREFIX (APPEND a c) (APPEND a b) = IS_PREFIX c b``,
+   Induct >> RW_TAC std_ss [APPEND]
+   ++ RW_TAC std_ss [APPEND, IS_PREFIX]);
+
+(*---------------------------------------------------------------------------
+        A well-formed encoder is prefix-free and injective.
+ ---------------------------------------------------------------------------*)
+
+val wf_encoder_def = Define
+  `wf_encoder e = !x y. IS_PREFIX (e x) (e y) ==> (x = y)`;
+
+(*---------------------------------------------------------------------------
+      The unit type is cool because it consumes no space in the
+      target list: the type has all the information!
+ ---------------------------------------------------------------------------*)
+
+val encode_unit_def =
+  TotalDefn.Define `encode_unit (_ : one) : bool list = []`;
 
 (*---------------------------------------------------------------------------
         Booleans
@@ -67,15 +118,15 @@ val (encode_num_def, encode_num_ind) =
     if n = 0 then [T; T]
     else if EVEN n then F :: encode_num ((n - 2) DIV 2)
     else T :: F :: encode_num ((n - 1) DIV 2)`,
-   TotalDefn.WF_REL_TAC `$<` THEN
-   REPEAT STRIP_TAC THEN
-   (KNOW_TAC (Term`?j. n = SUC j`) THEN1 ASM_MESON_TAC [num_CASES]) THEN
-   STRIP_TAC THEN
-   IMP_RES_TAC EVEN_EXISTS THEN
+   TotalDefn.WF_REL_TAC `$<` ++
+   REPEAT STRIP_TAC ++
+   (KNOW_TAC (Term `?j. n = SUC j`) >> PROVE_TAC [num_CASES]) ++
+   STRIP_TAC ++
+   IMP_RES_TAC EVEN_EXISTS ++
    ASM_SIMP_TAC arith_ss
-   [SUC_SUB1,MULT_DIV,DIV_LESS_EQ,
-    EQT_ELIM (ARITH_CONV (Term `2n*m - 2n = (m-1n)*2n`)),
-    EQT_ELIM (ARITH_CONV (Term `x < SUC y = x <= y`))]);
+   [SUC_SUB1, MULT_DIV, DIV_LESS_EQ,
+    DECIDE (Term `2n*m - 2n = (m-1n)*2n`),
+    DECIDE (Term `x < SUC y = x <= y`)]);
 
 val _ = save_thm ("encode_num_def", encode_num_def);
 val _ = save_thm ("encode_num_ind", encode_num_ind);
@@ -88,13 +139,121 @@ val _ = save_thm ("encode_num_ind", encode_num_ind);
        but then we'd need integers.
    ----------------------------------------------------------------------*)
 
-(*---------------------------------------------------------------------------
-      The unit type is cool because it consumes no space in the
-      target list: the type has all the information!
- ---------------------------------------------------------------------------*)
+(*---------------------------------------------------------------------------*)
+(* An alternative definition of encode_prod.                                 *)
+(*---------------------------------------------------------------------------*)
 
-val encode_unit_def =
-  TotalDefn.Define `encode_unit (_ : one) : bool list = []`;
+val encode_prod_alt = prove
+  (``!xb yb p. encode_prod xb yb p = APPEND (xb (FST p)) (yb (SND p))``,
+   GEN_TAC ++ GEN_TAC ++ Cases ++
+   RW_TAC std_ss [encode_prod_def]);
+
+(*---------------------------------------------------------------------------*)
+(* Proving that all our encoders are well-formed.                            *)
+(*---------------------------------------------------------------------------*)
+
+val wf_encode_unit = store_thm
+  ("wf_encode_unit",
+   ``wf_encoder encode_unit``,
+   RW_TAC std_ss [wf_encoder_def, encode_unit_def, IS_PREFIX, oneTheory.one]);
+
+val wf_encoder_bool = store_thm
+  ("wf_encoder_bool",
+   ``wf_encoder encode_bool``,
+   RW_TAC std_ss [wf_encoder_def, encode_bool_def, IS_PREFIX]);
+   
+val wf_encoder_prod = store_thm
+  ("wf_encoder_prod",
+   ``!f g. wf_encoder f /\ wf_encoder g ==> wf_encoder (encode_prod f g)``,
+   RW_TAC std_ss [wf_encoder_def, encode_prod_alt] ++
+   Cases_on `x` ++
+   Cases_on `y` ++
+   FULL_SIMP_TAC std_ss [] ++
+   Suff `q = q'` >> PROVE_TAC [IS_PREFIX_APPENDS] ++
+   PROVE_TAC [IS_PREFIX_APPEND1, IS_PREFIX_APPEND2]);
+
+val wf_encoder_sum = store_thm
+  ("wf_encoder_sum",
+   ``!f g. wf_encoder f /\ wf_encoder g ==> wf_encoder (encode_sum f g)``,
+   RW_TAC std_ss [wf_encoder_def] ++
+   Cases_on `x` ++
+   Cases_on `y` ++
+   FULL_SIMP_TAC std_ss [encode_sum_def, IS_PREFIX]);
+
+val wf_encoder_option = store_thm
+  ("wf_encoder_option",
+   ``!f. wf_encoder f ==> wf_encoder (encode_option f)``,
+   RW_TAC std_ss [wf_encoder_def] ++
+   Cases_on `x` ++
+   Cases_on `y` ++
+   FULL_SIMP_TAC std_ss [encode_option_def, IS_PREFIX]);
+
+val wf_encoder_num = store_thm
+  ("wf_encoder_num",
+   ``wf_encoder encode_num``,
+   SIMP_TAC std_ss [wf_encoder_def] ++
+   recInduct encode_num_ind ++
+   GEN_TAC ++
+   Cases_on `n = 0` >>
+   (POP_ASSUM SUBST1_TAC ++
+    SIMP_TAC std_ss [REWRITE_RULE [] (Q.INST [`n` |-> `0`] encode_num_def)] ++
+    ONCE_REWRITE_TAC [encode_num_def] ++
+    RW_TAC std_ss [IS_PREFIX]) ++
+   ASM_REWRITE_TAC [] ++
+   MP_TAC encode_num_def ++
+   (DISCH_THEN (fn th => RW_TAC std_ss [th]) ++
+    POP_ASSUM MP_TAC ++
+    Q.SPEC_TAC (`y`, `y`) ++
+    recInduct encode_num_ind ++
+    GEN_TAC ++
+    MP_TAC (Q.INST [`n` |-> `n'`] encode_num_def) ++
+    RW_TAC std_ss [IS_PREFIX] ++
+    RES_TAC) <<
+   [Cases_on `n` >> RW_TAC std_ss [] ++
+    Cases_on `n''` >> FULL_SIMP_TAC std_ss [EVEN] ++
+    FULL_SIMP_TAC arith_ss [EVEN] ++
+    Q.PAT_ASSUM `EVEN n` MP_TAC ++
+    RW_TAC std_ss [EVEN_EXISTS] ++
+    Cases_on `n'` >> RW_TAC std_ss [] ++
+    Cases_on `n` >> FULL_SIMP_TAC std_ss [EVEN] ++
+    FULL_SIMP_TAC arith_ss [EVEN] ++
+    Q.PAT_ASSUM `EVEN n'` MP_TAC ++
+    RW_TAC std_ss [EVEN_EXISTS] ++
+    POP_ASSUM MP_TAC ++
+    POP_ASSUM_LIST (K ALL_TAC) ++
+    Know `!m : num. SUC (SUC m) - 2 = m` >> DECIDE_TAC ++
+    DISCH_THEN (fn th => REWRITE_TAC [th]) ++
+    ONCE_REWRITE_TAC [MULT_COMM] ++
+    RW_TAC arith_ss [MULT_DIV],
+    Cases_on `n` >> RW_TAC std_ss [] ++
+    FULL_SIMP_TAC arith_ss [EVEN] ++
+    Q.PAT_ASSUM `EVEN n''` MP_TAC ++
+    RW_TAC std_ss [EVEN_EXISTS] ++
+    Cases_on `n'` >> RW_TAC std_ss [] ++
+    FULL_SIMP_TAC arith_ss [EVEN] ++
+    Q.PAT_ASSUM `EVEN n` MP_TAC ++
+    RW_TAC std_ss [EVEN_EXISTS] ++
+    POP_ASSUM MP_TAC ++
+    POP_ASSUM_LIST (K ALL_TAC) ++
+    ONCE_REWRITE_TAC [MULT_COMM] ++
+    RW_TAC arith_ss [MULT_DIV]]);
+
+val wf_encoder_list = store_thm
+  ("wf_encoder_list",
+   ``!f. wf_encoder f ==> wf_encoder (encode_list f)``,
+   RW_TAC std_ss [wf_encoder_def] ++
+   POP_ASSUM MP_TAC ++
+   Q.SPEC_TAC (`y`, `y`) ++
+   Q.SPEC_TAC (`x`, `x`) ++
+   Induct >>
+   (Cases ++
+    RW_TAC std_ss [IS_PREFIX, encode_list_def]) ++
+   GEN_TAC ++
+   Cases >> RW_TAC std_ss [IS_PREFIX, encode_list_def] ++
+   SIMP_TAC std_ss [encode_list_def, IS_PREFIX] ++
+   STRIP_TAC ++
+   Suff `h = h'` >> PROVE_TAC [IS_PREFIX_APPENDS] ++
+   PROVE_TAC [IS_PREFIX_APPEND1, IS_PREFIX_APPEND2]);
 
 (*---------------------------------------------------------------------------*)
 (* A congruence rule for encode_list                                         *)
@@ -106,11 +265,11 @@ val encode_list_cong = store_thm
       (l1=l2) /\ (!x. MEM x l2 ==> (f1 x = f2 x)) 
               ==>
       (encode_list f1 l1 = encode_list f2 l2)``,
-  Induct THEN SIMP_TAC list_ss [MEM,encode_list_def]
-         THEN RW_TAC list_ss []);
+  Induct ++
+  SIMP_TAC list_ss [MEM,encode_list_def] ++
+  RW_TAC list_ss []);
 
 val _ = DefnBase.write_congs (encode_list_cong::DefnBase.read_congs());
-
 
 val _ = adjoin_to_theory
 {sig_ps = NONE,
